compactness: more bumping

FOL_Compactness/Bumping.thy
@@ -43,7 +43,7 @@ fun bump_form :: "form \<Rightarrow> form" where
 
 find_theorems "_::nterm" name: induct
 
-lemma bumpterm: \<open>eval t \<M> \<beta> = eval (bump_nterm t) (bump_intrp \<M>) \<beta>\<close>
+lemma bumpterm: \<open>\<lbrakk>t\<rbrakk>\<^bsup>\<M>,\<beta>\<^esup> = \<lbrakk>bump_nterm t\<rbrakk>\<^bsup>bump_intrp \<M>,\<beta>\<^esup>\<close>
 proof (induct t)
   case (Var x)
   then show ?case
@@ -95,53 +95,178 @@ next
     by simp
 qed
 
-(* let FUNCTIONS_FORM_BUMPFORM = prove
- (`!p f m.
-        f,m IN functions_form(bumpform p)
-        ==> ?k. (f = NUMPAIR 0 k) /\ k,m IN functions_form p`, *)
 lemma functions_form_bumpform: \<open>(f, m) \<in> functions_form (bump_form \<phi>) \<Longrightarrow>
   \<exists>k. (f = numpair 0 k) \<and> (k, m) \<in> functions_form \<phi>\<close>
 proof (induct \<phi>)
+  case (Atom p ts)
+  then have \<open>\<exists>t\<in>set ts. (f, m) \<in> functions_term (bump_nterm t)\<close> by simp
+  then obtain t where t_in: \<open>t \<in> set ts\<close> and fm_in_t: \<open>(f, m) \<in> functions_term (bump_nterm t)\<close>
+      by blast
+  have \<open>\<exists>k. f = numpair 0 k \<and> (k, m) \<in> functions_term t\<close>
+    using fm_in_t
+  proof (induction t)
+    case (Var x)
+    then show ?case by auto
+  next
+    case (Fun g us)
+    find_theorems bump_nterm
+    have t_in_disj: \<open>functions_term (bump_nterm (Fun g us)) = 
+      {((numpair 0 g), length us)} \<union> (\<Union> u \<in> set us. functions_term (bump_nterm u))\<close>
+      by simp
+    then show ?case
+    proof (cases "(f, m) = ((numpair 0 g), length us)")
+      case True
+      then show ?thesis by auto
+    next
+      case False
+      then have \<open>(f, m) \<in> (\<Union> u \<in> set us. functions_term (bump_nterm u))\<close>
+        using t_in_disj
+        using Fun.prems by blast
+      then show ?thesis
+        using Fun(1) by fastforce
+    qed
+  qed
+  then have \<open>\<exists>k. f = numpair 0 k \<and> (\<exists>x\<in>set ts. (k, m) \<in> functions_term x)\<close>
+    using t_in by blast
+  then show ?case using Atom by simp
+qed auto
+
+lemma bumpform_interpretation: \<open>is_interpretation (language {\<phi>}) \<M> \<Longrightarrow>
+  is_interpretation (language {(bump_form \<phi>)}) (bump_intrp \<M>)\<close>
+  unfolding is_interpretation_def language_def by (meson FN_dom_to_dom list_all_set)
+
+(* unbumpterm in hol-light *)
+fun unbump_nterm :: "nterm \<Rightarrow> nterm" where
+  \<open>unbump_nterm (Var x) = Var x\<close>
+| \<open>unbump_nterm (Fun f ts) = Fun (numsnd f) (map unbump_nterm ts)\<close>
+
+(* unbumpform in hol-light *)
+fun unbump_form :: "form \<Rightarrow> form" where
+  \<open>unbump_form \<^bold>\<bottom> = \<^bold>\<bottom>\<close>
+| \<open>unbump_form (Atom p ts) = Atom p (map unbump_nterm ts)\<close>
+| \<open>unbump_form (\<phi> \<^bold>\<longrightarrow> \<psi>) = (unbump_form \<phi>) \<^bold>\<longrightarrow> (unbump_form \<psi>)\<close>
+| \<open>unbump_form (\<^bold>\<forall> x\<^bold>. \<phi>) = \<^bold>\<forall> x\<^bold>. (unbump_form \<phi>)\<close>
+
+lemma unbumpterm [simp]: "unbump_nterm (bump_nterm t) = t"
+  by (induct t) (simp add: list.map_ident_strong)+
+
+lemma unbumpform [simp]: \<open>unbump_form (bump_form \<phi>) = \<phi>\<close>
+  by (induct \<phi>) (simp add: list.map_ident_strong)+
+
+(* unbumpmod in hol-light *)
+definition unbump_intrp :: "'m intrp \<Rightarrow> 'm intrp" where
+  \<open>unbump_intrp \<M> = Abs_intrp (dom \<M>, (\<lambda>k zs. (intrp_fn \<M>) (numpair 0 k) zs), (intrp_rel \<M>))\<close>
+
+(* UNBUMPMOD_TERM in hol-light *)
+lemma unbump_term_intrp: \<open>\<lbrakk>bump_nterm t\<rbrakk>\<^bsup>\<M>,\<beta>\<^esup> = \<lbrakk>t\<rbrakk>\<^bsup>unbump_intrp \<M>,\<beta>\<^esup>\<close>
+proof (induct t)
+  case (Fun f ts)
+  then show ?case 
+    unfolding unbump_intrp_def
+    by (smt (verit, best) bump_nterm.simps(2) concat_map eval.simps(2) intrp_fn_Abs_is_fst_snd 
+        intrp_is_struct list.map_cong0 struct_def)
+qed simp
+
+(*  UNBUMPMOD in hol-light *)
+lemma unbump_holds: \<open>(\<M>,\<beta> \<Turnstile> bump_form \<phi>) = (unbump_intrp \<M>,\<beta> \<Turnstile> \<phi>)\<close>
+proof (induct \<phi> arbitrary: \<beta>)
   case Bot
   then show ?case
     by auto
 next
   case (Atom p ts)
-  {
-    assume \<open>\<exists>x\<in>set ts. (f, m) \<in> functions_term (bump_nterm x)\<close>
-    then obtain t where t_in: \<open>t \<in> set ts\<close> and fm_in_t: \<open>(f, m) \<in> functions_term (bump_nterm t)\<close>
-      by blast
-    have \<open>\<exists>k. f = numpair 0 k \<and> (k, m) \<in> functions_term t\<close>
-      using fm_in_t
-    proof (induction t)
-      case (Var x)
-      then show ?case by auto
-    next
-      case (Fun g us)
-      then show ?case
-      proof (cases "(f, m) = (g, length us)")
-        case True
-        then show ?thesis 
-          
-          sorry
-      next
-        case False
-        then show ?thesis sorry
-      qed
-    qed
-    then have \<open>\<exists>k. f = numpair 0 k \<and> (\<exists>x\<in>set ts. (k, m) \<in> functions_term x)\<close>
-      using t_in by blast
-  }
-  then show ?case using Atom by simp
+  then show ?case
+    unfolding unbump_intrp_def
+    by (smt (verit) bump_intrp_def bumpform dom_Abs_is_fst functions_form_bumpform
+        holds_indep_intrp_if intrp_fn_Abs_is_fst_snd intrp_is_struct intrp_rel_Abs_is_snd_snd
+        numsnd_simp struct_def)
 next
   case (Implies \<phi>1 \<phi>2)
-  then show ?case 
-    by auto
-next
-  case (Forall x1 \<phi>)
   then show ?case
     by auto
+next
+  case (Forall x \<phi>)
+  then show ?case
+    by (smt (verit, best) bump_form.simps(4) dom_Abs_is_fst holds.simps(4) intrp_is_struct 
+        struct_def unbump_intrp_def)
 qed
+
+fun numlist :: "nat list \<Rightarrow> nat" where
+  \<open>numlist [] = 0\<close>
+| \<open>numlist (n # ls) = numpair n ((numlist ls) + 1) \<close>
+
+lemma numlist_pos: \<open>l \<noteq> [] \<Longrightarrow> numlist l > 0\<close>
+proof (induct l)
+  case Nil
+  then show ?case by blast
+next
+  case (Cons a l)
+  then show ?case
+    using numpair_def by auto
+qed
+
+lemma numlist_inj: \<open>(numlist l1 = numlist l2) \<equiv> (l1 = l2)\<close>
+proof (induction l1 l2 rule: list_induct2')
+  case 1
+  then show ?case
+    by blast
+next
+  case (2 x xs)
+  then show ?case
+    using numlist_pos by force
+next
+  case (3 y ys)
+  then show ?case
+    using numlist_pos by force
+next
+  case (4 x xs y ys)
+  then show ?case
+    by (metis Suc_eq_plus1 nat.simps(1) numlist.simps(2) numpair_inj)
+qed
+
+fun num_of_term :: "nterm \<Rightarrow> nat" where
+  \<open>num_of_term (Var x) = numpair 0 x\<close>
+| \<open>num_of_term (Fun f ts) = numpair 1 (numpair f (numlist (map num_of_term ts)))\<close>
+
+(* to move in AFP theory First-Order Terms.Term *)
+lemma term_induct2: "(\<And>x y. P (Var x) (Var y)) \<Longrightarrow> (\<And>x g us. P (Var x) (Fun g us))
+   \<Longrightarrow> (\<And>f ts y. P (Fun f ts) (Var y)) \<Longrightarrow> (\<And>f ts g us. P (Fun f ts) (Fun g us))
+   \<Longrightarrow> P t1 t2"
+  by (metis term.collapse(1) term.collapse(2))
+
+lemma term_induct2': "(\<And>x y. P (Var x) (Var y)) \<Longrightarrow> (\<And>x g us. P (Var x) (Fun g us))
+   \<Longrightarrow> (\<And>f ts y. P (Fun f ts) (Var y))
+   \<Longrightarrow> (\<And>f ts g us. list_all2 P ts us \<Longrightarrow> P (Fun f ts) (Fun g us))
+   \<Longrightarrow> P t1 t2"
+  sorry
+
+(************************************************)
+
+(*
+NUM_OF_TERM_INJ = prove
+ (`!s t. (num_of_term s = num_of_term t) = (s = t)`, *)
+lemma num_of_term_inj: \<open>num_of_term s = num_of_term t \<equiv> s = t\<close>
+proof (induction s t rule: term_induct2)
+  case (1 x y)
+  then show ?case
+    by (metis num_of_term.simps(1) numsnd_simp)
+next
+  case (2 x g us)
+  then show ?case
+    by (metis Term.term.simps(4) le_refl not_one_le_zero num_of_term.elims numpair_inj)
+next
+  case (3 f ts y)
+  then show ?case
+    by (metis Term.term.simps(4) not_one_le_zero num_of_term.elims numpair_inj order_refl)
+next
+  case (4 f ts g us)
+  then show ?case
+    apply simp
+    using numpair_inj
+    sorry
+qed
+
+
 
 
 
